leakage freedom

proof/Ring_ops_extract_ct.ec
@@ -190,6 +190,24 @@ module M(SC:Syscall_t) = {
     return (a);
   }
   
+  proc bn_set0 (a:W64.t Array32.t) : W64.t Array32.t = {
+    var aux: int;
+    var aux_0: W64.t;
+    
+    var i:int;
+    
+    leakages <- LeakFor(0,32) :: LeakAddr([]) :: leakages;
+    i <- 0;
+    while (i < 32) {
+      leakages <- LeakAddr([]) :: leakages;
+      aux_0 <- (W64.of_int 0);
+      leakages <- LeakAddr([i]) :: leakages;
+      a.[i] <- aux_0;
+      i <- i + 1;
+    }
+    return (a);
+  }
+  
   proc bn_set1 (a:W64.t Array32.t) : W64.t Array32.t = {
     var aux_0: int;
     var aux: W64.t;
@@ -732,11 +750,11 @@ module M(SC:Syscall_t) = {
   }
   
   proc rsample (byte_z:W64.t Array32.t) : int * W64.t Array32.t = {
-    var aux_1: bool;
-    var aux_0: int;
-    var aux: W64.t;
-    var aux_2: W8.t Array256.t;
-    var aux_3: W64.t Array32.t;
+    var aux_2: bool;
+    var aux_1: int;
+    var aux_0: W64.t;
+    var aux_3: W8.t Array256.t;
+    var aux: W64.t Array32.t;
     
     var i:int;
     var byte_p:W64.t Array32.t;
@@ -748,44 +766,47 @@ module M(SC:Syscall_t) = {
     byte_p <- witness;
     byte_q <- witness;
     leakages <- LeakAddr([]) :: leakages;
-    aux <- (W64.of_int 0);
-    q0 <- aux;
+    aux <@ bn_set0 (byte_p);
+    byte_p <- aux;
     leakages <- LeakAddr([]) :: leakages;
-    aux <- (W64.of_int 1);
-    q1 <- aux;
+    aux_0 <- (W64.of_int 0);
+    q0 <- aux_0;
     leakages <- LeakAddr([]) :: leakages;
-    aux_0 <- 0;
-    i <- aux_0;
+    aux_0 <- (W64.of_int 1);
+    q1 <- aux_0;
     leakages <- LeakAddr([]) :: leakages;
-    aux_1 <- (q0 = (W64.of_int 0));
-    z <- aux_1;
+    aux_1 <- 0;
+    i <- aux_1;
+    leakages <- LeakAddr([]) :: leakages;
+    aux_2 <- (q0 = (W64.of_int 0));
+    z <- aux_2;
     
     leakages <- LeakCond(z) :: LeakAddr([]) :: leakages;
     
     while (z) {
       leakages <- LeakAddr([]) :: leakages;
-      aux_2 <@ SC.randombytes_256 ((Array256.init (fun i_0 => get8
+      aux_3 <@ SC.randombytes_256 ((Array256.init (fun i_0 => get8
                                    (WArray256.init64 (fun i_0 => byte_p.[i_0]))
                                    i_0)));
       byte_p <-
       (Array32.init (fun i_0 => get64
-      (WArray256.init8 (fun i_0 => aux_2.[i_0])) i_0));
+      (WArray256.init8 (fun i_0 => aux_3.[i_0])) i_0));
       leakages <- LeakAddr([]) :: leakages;
-      aux_3 <@ bn_copy (byte_p);
-      byte_q <- aux_3;
+      aux <@ bn_copy (byte_p);
+      byte_q <- aux;
       leakages <- LeakAddr([]) :: leakages;
-      (aux_1, aux_3) <@ bn_subc (byte_q, byte_z);
-      cf <- aux_1;
-      byte_q <- aux_3;
+      (aux_2, aux) <@ bn_subc (byte_q, byte_z);
+      cf <- aux_2;
+      byte_q <- aux;
       leakages <- LeakAddr([]) :: leakages;
-      aux <- (cf ? q1 : q0);
-      q0 <- aux;
+      aux_0 <- (cf ? q1 : q0);
+      q0 <- aux_0;
       leakages <- LeakAddr([]) :: leakages;
-      aux_1 <- (q0 = (W64.of_int 1));
-      z <- aux_1;
+      aux_2 <- (q0 = (W64.of_int 0));
+      z <- aux_2;
       leakages <- LeakAddr([]) :: leakages;
-      aux_0 <- (i + 1);
-      i <- aux_0;
+      aux_1 <- (i + 1);
+      i <- aux_1;
     leakages <- LeakCond(z) :: LeakAddr([]) :: leakages;
     
     }
