proof/Uniform_distr_proof_ct.ec
@@ -1,3 +1,4 @@
+
 require import Ring_ops_extract_ct.
 require import JModel List Int AllCore.
 
@@ -63,10 +64,37 @@ qed.
 
 
 
+(* set0 LEAKAGES  *)
+op set0_prefix : leakages_t = LeakFor (0, 32) :: LeakAddr [] :: [].
+op set0_step (i : int) : leakages_t = LeakAddr [i] :: LeakAddr [] :: [].
+
+op set0_g (x : int) : leakages_t.
+axiom set0_g_comp_1 x : 0 <= x  => set0_g x = [].
+axiom set0_g_comp_2 x : 0 < x => set0_g x = set0_step (x-1) ++ set0_g (x - 1).
+
+op set0_f (x : int) : leakages_t = set0_g x ++ set0_prefix.
+
+lemma bn_set0_leakages start_l :
+   hoare [ M(Syscall).bn_set0 : M.leakages = start_l ==> M.leakages = set0_f 32 ++ start_l ].
+proof. 
+proc.
+sp.  elim*. progress.
+conseq (_: M.leakages = set0_prefix ++ start_l /\ i = 0 ==> _).
+progress. rewrite /set0_prefix.
+while (0 <= i /\ i <= 32 /\ M.leakages = set0_f i ++ start_l).
+wp.  skip.  progress. 
+simplify. smt(). smt(). rewrite /set0_f. rewrite (set0_g_comp_2 (i{hr} +1)).  smt(). simplify. rewrite /set0_step. simplify. auto.
+skip. progress. rewrite /set0_f.  rewrite set0_g_comp_1. auto. auto. 
+smt().
+qed.
+
+
+
 (* SAMPLING LEAKAGES  *)
 op samp_prefix : leakages_t = 
   LeakCond true :: LeakAddr [] :: LeakAddr [] :: LeakAddr [] :: LeakAddr [] :: 
-  LeakAddr [] :: [].
+   LeakAddr [] :: (set0_f 32 ++ [LeakAddr []]).
+
 op samp_g (x : int) : leakages_t.
 op samp_step (i : int) : leakages_t = LeakCond true :: LeakAddr [] :: LeakAddr [] :: LeakAddr [] :: LeakAddr [] :: (
 sub_f 32 ++
@@ -91,9 +119,9 @@ op samp_t (x : int) : leakages_t = samp_suffix ++ samp_f (x - 1).
 lemma rsample_leakages :
    hoare [ M(Syscall).rsample : M.leakages = [] ==> M.leakages = samp_t res.`1].
 proc.
-sp. elim*. progress.
-conseq (_: M.leakages = samp_prefix /\ i = 0  /\ z = true ==> _).
-progress.
+seq 18 :  (M.leakages = samp_prefix /\ i = 0  /\ z = true ).
+wp. ecall (bn_set0_leakages M.leakages). wp. skip. progress. 
+
 while (0 <= i /\ (z = true => M.leakages = samp_f i) 
               /\ (z = false => M.leakages = samp_t i)).
 wp. 
@@ -111,7 +139,188 @@ rewrite H2. rewrite H. auto.
 auto.
 qed.
     
+require Ring_ops_extract.
+import Ring_ops_extract.
 
- (* show that M(syscall) ~ CSpec
+module M1 = Ring_ops_extract_ct.M(Ring_ops_extract_ct.Syscall).
+module M2 = Ring_ops_extract.M(Ring_ops_extract.Syscall).
 
-  *)
+lemma aaaa :
+  equiv  [ M1.bn_set0 ~ M2.bn_set0 
+    : ={arg} ==> ={res}  ].
+proc. 
+while (={a,i}). wp. skip. progress. wp.  skip. progress. qed.
+
+  
+lemma aaa :
+  equiv  [ M1.rsample ~ M2.rsample 
+    : ={arg} ==> ={res}  ].
+proof. proc.  sim. call aaaa. wp.  skip. progress. qed.
+
+require import Ring_ops_proof.
+require import Ring_ops_spec.
+
+
+equiv rsample_cspec2:
+ M1.rsample ~ CSpecFp.rsample:
+  W64xN.valR byte_z{1} = a{2}
+  ==> W64xN.valR res{1}.`2 = res{2}.`2 /\ res{1}.`1 = res{2}.`1.
+transitivity M2.rsample 
+ (={arg} ==> ={res})
+ (W64xN.valR byte_z{1} = a{2}
+  ==> W64xN.valR res{1}.`2 = res{2}.`2 /\ res{1}.`1 = res{2}.`1).
+progress. smt(). progress.
+conseq aaa. 
+conseq rsample_cspec.
+qed.
+
+import W64xN.
+require import Distr.
+
+lemma samew a &m : 0%r < mu D (RSP (valR a)) =>
+  Pr[ M1.rsample(a) @ &m : true  ] = 1%r.
+progress.
+rewrite - (rsample_lossless (W64xN.valR a) &m _). auto. 
+byequiv.
+conseq rsample_cspec2. progress. progress. smt().
+qed.
+
+
+lemma zzz a i x &m : 
+  Pr[ M1.rsample(a) @ &m : res = (i,x)  ]
+   =   Pr[ CSpecFp.rsample(W64xN.valR a) @ &m : res = (i, W64xN.valR x)  ].
+byequiv.
+conseq rsample_cspec2. progress. progress. smt().
+smt(@W64xN). auto. auto.
+qed.
+
+
+lemma qq' a  &m : (glob M1){m} = [] =>
+  Pr[ M1.rsample(a) @ &m : M1.leakages <> samp_t res.`1 ] = 0%r.
+progress. byphoare (_: glob M1 = [] ==> _).
+hoare. simplify.
+conseq rsample_leakages. auto. auto. auto.
+qed.
+
+lemma qq a l x &m : (glob M1){m} = [] => 0%r < mu D (RSP (valR a)) =>
+  Pr[ M1.rsample(a) @ &m : M1.leakages = l  /\ res.`2 = x ]
+  = Pr[ M1.rsample(a) @ &m : l = samp_t res.`1 /\ res.`2 = x  ].
+move => m1p m2p.
+have pr1 :  Pr[ M1.rsample(a) @ &m : M1.leakages = samp_t res.`1   ] = 1%r.
+rewrite - (samew a &m).   auto.
+  have ->: Pr[Ring_ops_extract_ct.M(Ring_ops_extract_ct.Syscall).rsample(a) @ &m : true] 
+   = Pr[Ring_ops_extract_ct.M(Ring_ops_extract_ct.Syscall).rsample(a) @ &m : M1.leakages = samp_t res.`1 ] + Pr[Ring_ops_extract_ct.M(Ring_ops_extract_ct.Syscall).rsample(a) @ &m : M1.leakages <> samp_t res.`1  ]. rewrite Pr[mu_split (M1.leakages = samp_t res.`1) ]. simplify. auto. rewrite (qq' a &m). auto.
+simplify. auto.
+have pr2 :  Pr[ M1.rsample(a) @ &m : M1.leakages <> samp_t res.`1   ] = 0%r.
+byphoare (_:(glob M1){m} = (glob M1) ==> _). 
+hoare. simplify.
+conseq rsample_leakages. smt(). progress. auto.
+have -> :   Pr[ M1.rsample(a) @ &m : M1.leakages = l /\ res.`2 = x  ]
+ = Pr[ M1.rsample(a) @ &m : M1.leakages = samp_t res.`1 /\ M1.leakages = l /\ res.`2 = x ].
+rewrite Pr[mu_split (M1.leakages = samp_t res.`1) ].
+  have -> : Pr[M1.rsample(a) @ &m :
+   (M1.leakages = l /\ res.`2 = x) /\ M1.leakages <> samp_t res.`1] = 0%r. smt(@Distr). 
+   simplify. rewrite Pr[mu_eq]. progress. auto. 
+have -> : Pr[M1.rsample(a) @ &m : l = samp_t res.`1 /\ res.`2 = x] 
+  = Pr[M1.rsample(a) @ &m : l = samp_t res.`1 /\ M1.leakages = samp_t res.`1 /\ res.`2 = x  ].
+rewrite Pr[mu_split (M1.leakages = samp_t res.`1) ].
+  have -> : Pr[M1.rsample(a) @ &m :
+   (l = samp_t res.`1 /\ res.`2 = x) /\ M1.leakages <> samp_t res.`1] = 0%r. smt(@Distr).  auto. 
+   simplify. rewrite Pr[mu_eq]. progress. auto. 
+rewrite Pr[mu_eq]. progress. auto.
+qed.
+
+require import InvFun.
+
+
+lemma samp_t_inj : injective samp_t.
+admitted.
+
+
+    
+lemma qqq a x l &m : (glob M1){m} = [] => 0%r < mu D (RSP (valR a)) =>
+  Pr[ M1.rsample(a) @ &m : M1.leakages = l  /\ res.`2 = x  ]
+  = Pr[ M1.rsample(a) @ &m :  (inv (-1) samp_t) l = res.`1  /\ res.`2 = x  ].
+move => ic ic'. rewrite  (qq a  l x &m). auto. auto.
+simplify. 
+have -> : 
+  Pr[Ring_ops_extract_ct.M(Ring_ops_extract_ct.Syscall).rsample(a) @ &m :
+   l = samp_t res.`1 /\ res.`2 = x]
+  =   Pr[Ring_ops_extract_ct.M(Ring_ops_extract_ct.Syscall).rsample(a) @ &m :
+   l = samp_t res.`1 /\ res.`2 = x /\ 0 <= res.`1]. byequiv.
+proc. wp. simplify.
+while (0 <= i{1} /\ ={i,byte_p, byte_z, q0, q1}). wp.  simplify.
+call (_:true). wp. sim. wp. 
+call (_:true). wp. sim. wp. 
+call (_:true). wp. sim. wp. 
+skip. progress. smt(). wp. 
+call (_:true). wp. sim. wp.  skip. progress.
+auto. auto.
+have -> : Pr[Ring_ops_extract_ct.M(Ring_ops_extract_ct.Syscall).rsample(a) @ &m :
+   inv (-1) samp_t l = res.`1 /\ res.`2 = x] 
+ = Pr[Ring_ops_extract_ct.M(Ring_ops_extract_ct.Syscall).rsample(a) @ &m :
+   inv (-1) samp_t l = res.`1 /\ res.`2 = x /\ 0 <= res.`1].
+ byequiv.
+proc. wp. simplify.
+while (0 <= i{1} /\ ={i,byte_p, byte_z, q0, q1}). wp.  simplify.
+call (_:true). wp. sim. wp. 
+call (_:true). wp. sim. wp. 
+call (_:true). wp. sim. wp. 
+skip. progress. smt(). wp. 
+call (_:true). wp. sim. wp.  skip. progress.
+auto. auto.
+rewrite Pr[mu_eq].
+progress.
+rewrite invP. apply samp_t_inj. auto.  
+have : exists z, (samp_t z) = l.
+apply (choiceEx (-1) samp_t l res{hr}.`1) . apply H. smt().
+elim. progress.
+rewrite - H.
+rewrite invP.
+apply samp_t_inj. auto.
+auto.
+qed.
+
+
+
+
+lemma ph_l5''_var &m a : Pr[M1.rsample(a) @ &m : res.`1 <= 0 ] = 0%r.
+byphoare (_: arg = a ==> _);auto. hoare.
+proc.  simplify.
+unroll 19. rcondt 19. wp. wp. 
+call (_:true). wp. auto. wp. skip. auto.
+while (0 < i). wp. call (_:true). auto. wp.  call (_:true). auto.  wp. 
+inline*. wp. rnd. wp. skip. progress. smt().
+wp. call (_:true). auto.  wp.  
+call (_:true). auto. wp. 
+call (_:true). auto. wp. 
+call (_:true). auto. wp. skip. smt().
+qed.
+
+
+op z a x l : real 
+ = if inv (-1) samp_t l <= 0 then 0%r else mu D (predC (RSP ((valR a)))) ^ (inv (-1) samp_t l - 1) *
+        (mu1 D ((valR x))).
+
+lemma leakfree &m x a l: (glob M1){m} = [] => valR x < valR a => 0%r < mu D (RSP (valR a)) =>
+  Pr[ M1.rsample(a) @ &m : M1.leakages = l  /\ res.`2 = x  ]
+    = z a x l.
+      progress.
+   rewrite  (qqq a x l &m);auto.
+case (inv (-1) samp_t l <= 0). 
+move => q. rewrite /z. rewrite q.  simplify. 
+  have : Pr[Ring_ops_extract_ct.M(Ring_ops_extract_ct.Syscall).rsample(a) @ &m :
+   inv (-1) samp_t l = res.`1 /\ res.`2 = x] 
+    <= Pr[M1.rsample(a) @ &m : res.`1 <= 0 ]. simplify. rewrite Pr[mu_sub]. smt().
+   auto. smt(ph_l5''_var @Distr).
+move => q.
+have -> : 
+ Pr[Ring_ops_extract_ct.M(Ring_ops_extract_ct.Syscall).rsample(a) @ &m :
+   inv (-1) samp_t l = res.`1 /\ res.`2 = x]
+  = Pr[Ring_ops_extract_ct.M(Ring_ops_extract_ct.Syscall).rsample(a) @ &m :
+   res = (inv (-1) samp_t l , x) ]. rewrite Pr[mu_eq]. smt(). auto.
+rewrite zzz.
+rewrite rsample_pr.   smt().
+rewrite /RSP. auto.
+rewrite /z. smt().
+qed.
